\begin{wideslide}[bm=,toc=]{\large Semantics of Propositional Operators}
\begin{center}
\begin{tabular}{|c|c|c|c|}
\hline
$A$ & $v(A_{1})$ & $v(A_{2})$ & $v(A)$ \\ \hline \hline
$\ngg A_{1}$ & $T$ & & $F$  \\
$\ngg A_{1}$ & $F$ & & $T$ \\ \hline
$A_{1} \vee A_{2}$ & $F$ & $F$ & $F$ \\
$A_{1} \vee A_{2}$ & \multicolumn{2}{c|}{otherwise}  & $T$ \\ \hline
$A_{1} \wedge A_{2}$ & $T$ & $T$ & $T$ \\
$A_{1} \wedge A_{2}$ & \multicolumn{2}{c|}{otherwise}  & $F$ \\ \hline
$A_{1} \imp A_{2}$ & $T$ & $F$ & $F$ \\
$A_{1} \imp  A_{2}$ &
   \multicolumn{2}{c|}{otherwise}  & $T$ \\ \hline
$A_{1} \eqv A_{2}$ & \multicolumn{2}{c|}{$v(A_{1})=v(A_{2})$} & $T$ \\
$A_{1} \eqv A_{2}$ & \multicolumn{2}{c|}{$v(A_{1})\neq v(A_{2})$} &
  $F$ \\ \hline
\end{tabular}
\end{center}
\end{wideslide}

\begin{wideslide}[bm=,toc=]{\large Wason Selection Task}
\begin{center}
\begin{picture}(290,20)
\put(0,0){\framebox(50,20){$p3$}}
\put(80,0){\framebox(50,20){$p5$}}
\put(160,0){\framebox(50,20){$\mathit{flag}=1$}}
\put(240,0){\framebox(50,20){$\mathit{flag}=0$}}
\end{picture}
\end{center}
\end{wideslide}

\begin{wideslide}[bm=,toc=]{\large }
\begin{alg}{Verification example}{integer x1, integer x2}
\decl{integer y1 \la{} 0, integer y2 \la{} 0, integer y3}\hline
\stt{read(x1,x2)}
\stt{y3 \la{} x1}
\stt{while y3 $\neq$ 0}
\stt{\idt{}if y2$+$1 $=$ x2}
\stt{\idt{}\idt{}y1 \la{} y1 $+$ 1}
\stt{\idt{}\idt{}y2 \la{} 0}
\stt{\idt{}else}
\stt{\idt{}\idt{}y2 \la{} y2 $+$ 1}
\stt{\idt{}y3 \la{} y3 $-$ 1}
\stt{write(y1,y2)}
\end{alg}
\end{wideslide}

\begin{wideslide}[bm=,toc=]{\large Spark Program for Integer Division}
\program{Spark}{Divide.ada}
\end{wideslide}

\begin{wideslide}[bm=,toc=]{\large Integer Division}
\program{Spark}{Divide1.ada}
\end{wideslide}

\begin{wideslide}[bm=,toc=]{\large Verification Conditions for Integer Division}
\textsf{Precondition to assertion:}
\begin{displaymath}
\begin{array}{l}
(X1 \geq 0) \wedge (X2 > 0) \: \imp \: \\
(X1 = Q \cdot X2 + R + N) \wedge (X2 > R) \wedge (R \geq 0).
\end{array}
\end{displaymath}
\textsf{Assertion to postcondition:}
\begin{displaymath}
\begin{array}{l}
(X1 = Q \cdot X2 + R + N) \wedge (X2 > R) \wedge (R \geq 0)
\wedge (N = 0) \:\imp\:\\
(X1 = Q \cdot X2 + R) \wedge (X2 > R) \wedge (R \geq 0).
\end{array}
\end{displaymath}
\textsf{Assertion to assertion by \textsf{then} branch:}
\begin{displaymath}
\begin{array}{l}
(X1 = Q \cdot X2 + R + N) \wedge (X2 > R) \wedge (R \geq 0)
\wedge (R+1 = X2) \:\imp\:\\
(X1 = Q' \cdot X2 + R' + N') \wedge (X2 > R') \wedge (R' \geq 0).
\end{array}
\end{displaymath}
\textsf{Assertion to assertion by \textsf{else} branch:}
\begin{displaymath}
\begin{array}{l}
(X1 = Q \cdot X2 + R + N) \wedge (X2 > R) \wedge (R \geq 0)
\wedge (R+1 \neq X2) \:\imp\:\\
(X1 = Q' \cdot X2 + R' + N') \wedge (X2 > R') \wedge (R' \geq 0).
\end{array}
\end{displaymath}
\end{wideslide}
